fairneris/aneris_lang/aneris_lang.v
@@ -1,5 +1,5 @@
 From fairneris.aneris_lang Require Export lang.
 
-Canonical Structure aneris_ectxi_lang := EctxiLanguage head_step config_step locale_of aneris_lang_mixin.
+Canonical Structure aneris_ectxi_lang := EctxiLanguage head_step config_step locale_of config_enabled aneris_lang_mixin.
 Canonical Structure aneris_ectx_lang := EctxLanguageOfEctxi aneris_ectxi_lang.
 Canonical Structure aneris_lang := LanguageOfEctx aneris_ectx_lang.
