fairneris/aneris_lang/base_lang.v
@@ -1,5 +1,5 @@
 From fairneris.aneris_lang Require Export lang.
 
-Canonical Structure base_ectxi_lang := EctxiLanguage base_lang.head_step base_config_step base_lang.locale_of base_mixin.
+Canonical Structure base_ectxi_lang := EctxiLanguage base_lang.head_step base_config_step base_lang.locale_of base_lang.base_config_enabled base_mixin.
 Canonical Structure base_ectx_lang := EctxLanguageOfEctxi base_ectxi_lang.
 Canonical Structure base_lang := LanguageOfEctx base_ectx_lang.
